Computability/Constructions/CovRec.lean
@@ -391,67 +391,6 @@ end mod
 
 
 
--- We define interpretations of naturals as finite strings on the alphabet {0,1}.
--- (l,b) is interpreted as the string of length l, whose sequence matches with the binary representation of b.
-
-section BSMem
-/-- `BSMem (x,(l,b)) = [x∈Dₐ]` (iversion brackets) -/
-def Nat.BSMem : ℕ→ℕ := fun xa => if Nat.testBit xa.r.r xa.l then 1 else 0
-theorem BSMem_eq_BSMem_aux : Nat.BSMem = fun xa => xa.r.r % (2^xa.l) := by sorry
-namespace Nat.RecursiveIn.Code
-
-#eval BSMem (Nat.pair 1 (Nat.pair 5 0b01000))
-#eval BSMem (Nat.pair 2 (Nat.pair 5 0b01000))
-#eval BSMem (Nat.pair 3 (Nat.pair 5 0b01000))
-
-def c_BSMem := c_mod.comp₂ (right.comp right) (c_pow.comp₂ (c_const 2) left)
-@[simp] theorem c_BSMem_ev_pr:code_prim c_BSMem := by repeat (first|assumption|simp|constructor)
-@[simp] theorem c_BSMem_evp:eval_prim O c_BSMem = Nat.BSMem := by
-  simp [c_BSMem,eval_prim]
-  rw [BSMem_eq_BSMem_aux]
-@[simp] theorem c_BSMem_ev:eval O c_BSMem = Nat.BSMem := by rw [← eval_prim_eq_eval c_BSMem_ev_pr]; simp only [c_BSMem_evp]
-end Nat.RecursiveIn.Code
-theorem Nat.PrimrecIn.BSMem:Nat.PrimrecIn O Nat.BSMem := by rw [← c_BSMem_evp]; apply code_prim_prop c_BSMem_ev_pr
-theorem Nat.Primrec.BSMem:Nat.Primrec Nat.BSMem := by exact PrimrecIn.PrimrecIn_Empty PrimrecIn.BSMem
-end BSMem
-
-section BSUnion
-def Nat.BSUnion : ℕ→ℕ := fun bl1bl2 => Nat.pair (Nat.max bl1bl2.l.l bl1bl2.r.l) (Nat.lor bl1bl2.l.r bl1bl2.r.r)
-theorem BSUnion_eq_BSUnion_aux : Nat.BSUnion = fun xa => xa.r.r % (2^xa.l) := by sorry
-namespace Nat.RecursiveIn.Code
-def c_BSUnion := c_mod.comp₂ (right.comp right) (c_pow.comp₂ (c_const 2) left)
-@[simp] theorem c_BSUnion_ev_pr:code_prim c_BSUnion := by repeat (first|assumption|simp|constructor)
-@[simp] theorem c_BSUnion_evp:eval_prim O c_BSUnion = Nat.BSUnion := by
-  simp [c_BSUnion,eval_prim]
-  rw [BSUnion_eq_BSUnion_aux]
-@[simp] theorem c_BSUnion_ev:eval O c_BSUnion = Nat.BSUnion := by rw [← eval_prim_eq_eval c_BSUnion_ev_pr]; simp only [c_BSUnion_evp]
-end Nat.RecursiveIn.Code
-theorem Nat.PrimrecIn.BSUnion:Nat.PrimrecIn O Nat.BSUnion := by rw [← c_BSUnion_evp]; apply code_prim_prop c_BSUnion_ev_pr
-theorem Nat.Primrec.BSUnion:Nat.Primrec Nat.BSUnion := by exact PrimrecIn.PrimrecIn_Empty PrimrecIn.BSUnion
-end BSUnion
-
-section BSSize
-def Nat.BSSize : ℕ → ℕ
-| 0     => 0
-| (n+1) => (n+1)&&&1 + BSSize ((n+1)/2)
-theorem BSSize_eq_BSSize_aux : Nat.BSSize = fun xa => xa.r.r % (2^xa.l) := by sorry
-namespace Nat.RecursiveIn.Code
-
-
-
-def c_BSSize := c_mod.comp₂ (right.comp right) (c_pow.comp₂ (c_const 2) left)
-@[simp] theorem c_BSSize_ev_pr:code_prim c_BSSize := by repeat (first|assumption|simp|constructor)
-@[simp] theorem c_BSSize_evp:eval_prim O c_BSSize = Nat.BSSize := by
-  simp [c_BSSize,eval_prim]
-  rw [BSSize_eq_BSSize_aux]
-@[simp] theorem c_BSSize_ev:eval O c_BSSize = Nat.BSSize := by rw [← eval_prim_eq_eval c_BSSize_ev_pr]; simp only [c_BSSize_evp]
-end Nat.RecursiveIn.Code
-theorem Nat.PrimrecIn.BSSize:Nat.PrimrecIn O Nat.BSSize := by rw [← c_BSSize_evp]; apply code_prim_prop c_BSSize_ev_pr
-theorem Nat.Primrec.BSSize:Nat.Primrec Nat.BSSize := by exact PrimrecIn.PrimrecIn_Empty PrimrecIn.BSSize
-end BSSize
-
-
-
 
 
 section div2
@@ -813,6 +752,6 @@ theorem eval_replace_oracle_prop {O o c} (ho:code_total O o) : eval O (replace_o
 
 
 end Nat.RecursiveIn.Code
-theorem Nat.PrimrecIn.replace_oracle:Nat.PrimrecIn O (unpaired2 replace_oracle) := by rw [← c_replace_oracle_evp]; apply code_prim_prop c_replace_oracle_ev_pr
+theorem Nat.PrimrecIn.replace_oracle:Nat.PrimrecIn O (unpaired2 replace_oracle) := by rw [← c_replace_oracle_evp]; exact code_prim_prop
 theorem Nat.Primrec.replace_oracle:Nat.Primrec (unpaired2 replace_oracle) := by exact PrimrecIn.PrimrecIn_Empty PrimrecIn.replace_oracle
 end replace_oracle
