Computability/Oracle2.lean
@@ -1,0 +1,29 @@
+import Mathlib.Data.Nat.Pairing
+import Mathlib.Data.PFun
+import Mathlib.Computability.Partrec
+
+open Part
+
+namespace Nat
+
+inductive RecursiveIn (O : ℕ → ℕ) : (ℕ →. ℕ) → Prop
+  | zero : RecursiveIn O fun _ => 0
+  | succ : RecursiveIn O Nat.succ
+  | left : RecursiveIn O fun n => (Nat.unpair n).1
+  | right : RecursiveIn O fun n => (Nat.unpair n).2
+  | oracle : RecursiveIn O O
+  | pair {f h : ℕ →. ℕ} (hf : RecursiveIn O f) (hh : RecursiveIn O h) :
+      RecursiveIn O fun n => (Nat.pair <$> f n <*> h n)
+  | comp {f h : ℕ →. ℕ} (hf : RecursiveIn O f) (hh : RecursiveIn O h) :
+      RecursiveIn O fun n => h n >>= f
+  | prec {f h : ℕ →. ℕ} (hf : RecursiveIn O f) (hh : RecursiveIn O h) :
+      RecursiveIn O fun p =>
+        let (a, n) := Nat.unpair p
+        n.rec (f a) fun y IH => do
+          let i ← IH
+          h (Nat.pair a (Nat.pair y i))
+  | rfind {f : ℕ →. ℕ} (hf : RecursiveIn O f) :
+      RecursiveIn O fun a =>
+        Nat.rfind fun n => (fun m => m = 0) <$> f (Nat.pair a n)
+
+end Nat
